\documentclass{article}
\usepackage{amsmath}
\usepackage{amssymb}

\begin{document}

\section*{Proof: 3D DFT and IDFT can be computed by multi-pass 1D DFTs}

We begin with the 3D DFT definition:

\[
\Psi(f_x, f_y, f_t) = \sum_{x=0}^{w-1} \sum_{y=0}^{h-1} \sum_{t=0}^{n-1} \psi(x, y, t) \cdot e^{-j 2\pi \left( \frac{f_x x}{w} + \frac{f_y y}{h} + \frac{f_t t}{n} \right)}
\]

Because the exponential is separable, we can factor it:

\[
= \sum_{x=0}^{w-1} \sum_{y=0}^{h-1} \sum_{t=0}^{n-1} \psi(x, y, t) \cdot
e^{-j 2\pi \frac{f_t t}{n}} \cdot
e^{-j 2\pi \frac{f_y y}{h}} \cdot
e^{-j 2\pi \frac{f_x x}{w}}
\]

Rewriting the summation order by ppt:

\[
= \sum_{x=0}^{w-1} e^{-j 2\pi \frac{f_x x}{w}} 
\sum_{y=0}^{h-1} e^{-j 2\pi \frac{f_y y}{h}} 
\sum_{t=0}^{n-1} \psi(x, y, t) \cdot e^{-j 2\pi \frac{f_t t}{n}}
\]

We now define intermediate terms:

\begin{align*}
\psi_1(x, y, f_t) &= \sum_{t=0}^{n-1} \psi(x, y, t) \cdot e^{-j 2\pi \frac{f_t t}{n}} \\
\psi_2(x, f_y, f_t) &= \sum_{y=0}^{h-1} \psi_1(x, y, f_t) \cdot e^{-j 2\pi \frac{f_y y}{h}} \\
\Psi(f_x, f_y, f_t) &= \sum_{x=0}^{w-1} \psi_2(x, f_y, f_t) \cdot e^{-j 2\pi \frac{f_x x}{w}}
\end{align*}

\subsection*{Conclusion (DFT)}

Thus, the 3D DFT can be computed as three passes of 1D DFT:
\[
\psi(x, y, t) \xrightarrow{\text{1D DFT along } t} \psi_1(x, y, f_t)
\xrightarrow{\text{1D DFT along } y} \psi_2(x, f_y, f_t)
\xrightarrow{\text{1D DFT along } x} \Psi(f_x, f_y, f_t)
\]

\bigskip

Now consider the 3D inverse DFT:

\[
\psi(x, y, t) = \frac{1}{whn} \sum_{f_x=0}^{w-1} \sum_{f_y=0}^{h-1} \sum_{f_t=0}^{n-1} \Psi(f_x, f_y, f_t) \cdot e^{j 2\pi \left( \frac{f_x x}{w} + \frac{f_y y}{h} + \frac{f_t t}{n} \right)}
\]

This is also separable:

\[
= \frac{1}{whn} \sum_{f_x=0}^{w-1} e^{j 2\pi \frac{f_x x}{w}}
\sum_{f_y=0}^{h-1} e^{j 2\pi \frac{f_y y}{h}}
\sum_{f_t=0}^{n-1} \Psi(f_x, f_y, f_t) \cdot e^{j 2\pi \frac{f_t t}{n}}
\]

Define intermediate terms for IDFT:

\begin{align*}
\Psi_1(f_x, f_y, t) &= \sum_{f_t=0}^{n-1} \Psi(f_x, f_y, f_t) \cdot e^{j 2\pi \frac{f_t t}{n}} \\
\Psi_2(f_x, y, t) &= \sum_{f_y=0}^{h-1} \Psi_1(f_x, f_y, t) \cdot e^{j 2\pi \frac{f_y y}{h}} \\
\psi(x, y, t) &= \frac{1}{whn} \sum_{f_x=0}^{w-1} \Psi_2(f_x, y, t) \cdot e^{j 2\pi \frac{f_x x}{w}}
\end{align*}

\subsection*{Conclusion (IDFT)}

3D IDFT can also be computed by three successive 1D IDFTs:
\[
\Psi(f_x, f_y, f_t) \xrightarrow{\text{1D IDFT along } f_t} \Psi_1(f_x, f_y, t)
\xrightarrow{\text{1D IDFT along } f_y} \Psi_2(f_x, y, t)
\xrightarrow{\text{1D IDFT along } f_x} \psi(x, y, t)
\]

\end{document}
